Update equiv to work with extra fuel

src/CPS/Conversion.v
@@ -1,8 +1,9 @@
-Require Import FunInd.
+From Utils Require Import Env Tactics.
+From Common Require Import Literal Primitive.
 From Src Require Import Tree Fun_sem.
 From CPS Require Import Tree Fun_sem.
-From Common Require Import Literal Primitive.
-From Utils Require Import Env.
+(* Equi. *)
+Require Import FunInd.
 
 Open Scope list_scope.
 
@@ -11,140 +12,292 @@ Module SV := Src.Fun_sem.
 Module CT := CPS.Tree.
 Module CV := CPS.Fun_sem.
 
-Fixpoint cps_rec (nf: nat) (t: ST.term) (ctx: (nat * CT.atom) -> (nat * CT.term)): nat * CT.term :=
-  match t with 
-  | ST.Var n => ctx (nf, Var n)
-  | ST.Const l => ctx (nf, CT.Lit l)
-  | ST.Let x t rest => 
-      let (nf', rest') := cps_rec nf rest ctx in
-      cps_rec nf' t (fun r => 
-        let (nf'', n) := r in
-        (nf'', CT.LetU x Id n rest'))
-  | ST.LetRec (ST.Fnt fname farg fbody) rest =>
-      let retC := nf in
-      let (nf', fbody') := cps_rec (nf + 1) fbody (fun r => 
-        let (nf_f, f) := r in (nf_f, CT.AppC1 retC f)) in
-      let (nf'', rest') := cps_rec nf' rest ctx in 
-      (nf'', CT.LetF (Fnt fname retC farg fbody') rest')
+Function cps_rec (nf : nat) (t : ST.term) (cnt : nat) {struct t} : nat * CT.term :=
+  match t with
+  | ST.Var n => (nf, CT.AppC1 cnt (CT.Var n))
+  | ST.Const l => (nf, CT.AppC1 cnt (CT.Lit l))
+  | ST.Let n t r => 
+      let (nf, cb) := cps_rec nf r cnt in
+      let cn := nf in
+      let (nf, t') := cps_rec (nf + 1) t cn in
+      (nf, CT.LetC (CT.Cnt1 cn n cb) t')
+  | ST.LetRec (ST.Fnt n a b) r => 
+      let c := nf in 
+      let (nf, b') := cps_rec (nf + 1) b c in 
+      let (nf, r') := cps_rec nf r cnt in 
+      (nf, CT.LetF (CT.Fnt n c a b') r')
   | ST.App f t =>
-      let c := nf in
-      let carg := nf + 1 in
-      let (nf', cbody) := ctx (nf + 2, Var carg) in 
-      cps_rec nf' f (fun r => 
-        let (nf'', f') := r in
-        cps_rec nf'' t (fun r' => 
-          let (nf3, t') := r' in
-            (nf3, CT.LetC (Cnt1 c carg cbody) (AppF f' c t'))
-          )
-        )
+      let ct := nf in
+      let ta := nf + 1 in 
+      let af := nf + 2 in 
+      let bt := CT.AppF (CT.Var af) cnt (CT.Var ta) in (* Once f and t have been computer, we call f *)
+      let cntt := CT.Cnt1 ct ta bt in 
+      let (nf, t') := cps_rec (nf + 3) t ct in
+      let cf := nf in 
+      let bf := CT.LetC cntt t' in (* Once we are done computing f, we compute t *)
+      let cntf := CT.Cnt1 cf af bf in
+      let (nf, f') := cps_rec (nf + 1) f cf in
+      let res := CT.LetC cntf f' in 
+      (nf, res)
   | ST.In => 
-      let n := nf in
-      let (nf', r) := ctx (nf + 1, Var n) in
-      (nf', CT.LetIn n r)
+      let res := CT.LetIn nf (CT.AppC1 cnt (CT.Var nf)) in
+      (nf + 1, res)
   | ST.Out t => 
-      let n := nf in
-      let (nf', rest) := ctx (nf + 1, Var n) in
-      cps_rec nf' t (fun r => 
-        let (nf'', t') := r in 
-        (nf'', CT.LetOut n t' rest)
-      )
-  | ST.Ite cond thent elset => 
-      let c := nf in 
-      let carg := nf + 1 in 
-      let (nf', cbody) := ctx (nf + 2, Var carg) in 
-      let thenc := nf' in 
-      let (nf2, thent') := cps_rec (nf' + 1) thent (fun r => 
-        let (nf3, t) := r in 
-        (nf3, CT.AppC1 c t)
-      ) in 
-      let elsec := nf2 in
-      let (nf4, elset') := cps_rec (nf2 + 1) elset (fun r => 
-        let (nf5, t) := r in 
-        (nf5, CT.AppC1 c t)
-      ) in 
-      cps_rec nf4 cond (fun r => 
-        let (nf6, cond') := r in
-        (nf6, CT.LetC (Cnt1 c carg cbody) (
-          CT.LetC (Cnt0 thenc thent') (
-            CT.LetC (Cnt0 elsec elset') (
-              CT.Ite cond' thenc elsec
-            )
-          )
-        ))
-      )
-  | ST.BinaryOp op t1 t2 => 
-      let n := nf in
-      cps_rec (nf + 1) t1 (fun r => 
-        let (nf1, t1') := r in
-        cps_rec nf1 t2 (fun r' =>
-          let (nf2, t2') := r' in
-          let (nf3, t) := ctx (nf2, Var n) in
-          (nf3, CT.LetB n op t1' t2' t)
-        )  
-      )
-  | ST.UnaryOp op t =>
-      let n := nf in
-      cps_rec (nf + 1) t (fun r => 
-        let (nf1, t') := r in
-        let (nf2, rest) := ctx (nf1, Var n) in
-        (nf2, CT.LetU n op t' rest)
-      )
-  | ST.Match scrut (larg, lt) (rarg, rt) =>
-      let c := nf in 
-      let carg := nf + 1 in 
-      let (nf1, cbody) := ctx (nf + 2, Var carg) in 
-      let cnt := CT.Cnt1 c carg cbody in
-      let lc := nf1 in
-      let (nf2, lbody) := cps_rec (nf1 + 1) lt (fun r => 
-        let (nf3, lt') := r in
-        (nf3, CT.AppC1 c lt')
-      ) in
-      let lcnt := CT.Cnt1 lc larg lbody in
-      let rc := nf2 in
-      let (nf4, rbody) := cps_rec (nf2 + 1) rt (fun r =>
-        let (nf5, rt') := r in
-        (nf5, CT.AppC1 c rt')
-      ) in
-      let rcnt := CT.Cnt1 rc rarg rbody in
-      cps_rec nf4 scrut (fun r => 
-        let (nf6, scrut') := r in
-        (nf6, CT.LetC cnt (
-          CT.LetC lcnt (
-            CT.LetC rcnt (
-              CT.Match scrut' lc rc
-            )
-          )
-        ))
-      )
+      let c  := nf in 
+      let a := nf + 1 in 
+      let n := nf + 2 in 
+      let b := CT.LetOut n (CT.Var a) (CT.AppC1 cnt (CT.Var n)) in
+      let (nf, t') := cps_rec (nf + 3) t c in
+      let res := CT.LetC (CT.Cnt1 c a b) t' in 
+      (nf, res)
+  | ST.Ite c t e => 
+      let ct := nf in 
+      let (nf, bt) := cps_rec (nf + 1) t cnt in 
+      let cntt := CT.Cnt0 ct bt in
+      let ce := nf in 
+      let (nf, be) := cps_rec (nf + 1) e cnt in 
+      let cnte := CT.Cnt0 ce be in
+      let cc := nf in
+      let ac := nf + 1 in
+      let bc := CT.LetC cntt (CT.LetC cnte (CT.Ite (CT.Var ac) ct ce)) in 
+      let cntc := CT.Cnt1 cc ac bc in
+      let (nf, c') := cps_rec (nf + 2) c cc in 
+      let res := CT.LetC cntc c' in 
+      (nf, res)
+  | ST.BinaryOp op t1 t2 =>
+      let c2 := nf in 
+      let a2 := nf + 1 in
+      let a1 := nf + 2 in
+      let n := nf + 3 in 
+      let b2 := CT.LetB n op (CT.Var a1) (CT.Var a2) (CT.AppC1 cnt (CT.Var n)) in
+      let cnt2 := CT.Cnt1 c2 a2 b2 in
+      let (nf, t2') := cps_rec (nf + 4) t2 c2 in
+      let c1 := nf in
+      let b1 := CT.LetC cnt2 t2' in 
+      let cnt1 := CT.Cnt1 c1 a1 b1 in (* When t1 is computed, we compute t2 *)
+      let (nf, t1') := cps_rec (nf + 1) t1 c1 in
+      let res := CT.LetC cnt1 t1' in
+      (nf, res)
+  | ST.UnaryOp op t => 
+      let c := nf in
+      let a := nf + 1 in 
+      let n := nf + 2 in 
+      let b := CT.LetU n op (CT.Var a) (CT.AppC1 cnt (CT.Var n)) in 
+      let cntt := CT.Cnt1 c a b in
+      let (nf, t') := cps_rec (nf + 3) t c in 
+      let res := CT.LetC cntt t' in
+      (nf, res)
+  | ST.Match s (la, lt) (ra, rt) => 
+      let cl := nf in 
+      let (nf, lt') := cps_rec (nf + 1) lt cnt in
+      let cntl := CT.Cnt1 cl la lt' in 
+      let cr := nf in 
+      let (nf, rt') := cps_rec (nf + 1) rt cnt in 
+      let cntr := CT.Cnt1 cr ra rt' in
+      let cs := nf in
+      let sa := nf + 1 in
+      let sb := CT.LetC cntl (CT.LetC cntr (CT.Match (CT.Var sa) cl cr)) in 
+      let cnts := CT.Cnt1 cs sa sb in 
+      let (nf, s') := cps_rec (nf + 2) s cs in 
+      let res := CT.LetC cnts s' in 
+      (nf, res)
   end.
 
-Fixpoint cps_rec_v (nf : nat) (v : SV.value) {struct v} : nat * CV.value :=
+Create HintDb cps.
+
+Ltac cps_rec_nf_monotone_ind IH := 
+  match goal with
+  | H : cps_rec ?nf ?t ?c = (?nf', ?t') |- _ => 
+         eapply IH in H; auto with lia
+  end.
+
+Lemma cps_rec_nf_monotone_size : forall n t cnt nf nf' t', ST.size t < n -> 
+  cps_rec nf t cnt = (nf', t') -> nf <= nf'.
+Proof with eauto with lia.
+  induction n, t...
+  all: repeat reduce || destruct_match || cps_rec_nf_monotone_ind IHn...
+Qed.
+
+Lemma cps_rec_nf_monotone : forall nf t cnt nf' t', 
+  cps_rec nf t cnt = (nf', t') -> nf <= nf'.
+Proof.
+  eauto using cps_rec_nf_monotone_size.
+Qed.
+
+#[global]
+Hint Resolve cps_rec_nf_monotone : cps.
+
+Ltac cps_rec_nf_correct_ind IH := 
+  match goal with
+  | H : cps_rec ?nf ?t ?c = (?nf', ?t') |- _ => 
+        pose proof (cps_rec_nf_monotone _ _ _ _ _ H);
+        eapply IH in H; auto with lia; [idtac]
+  end.
+
+Opaque Nat.max.
+
+Lemma cps_rec_nf_correct_size : forall n t cnt nf nf' t', ST.size t < n -> 
+  ST.next_free t <= nf -> cnt < nf ->
+  cps_rec nf t cnt = (nf', t') -> CT.next_free t' <= nf'.
+Proof with auto with lia cps.
+  induction n, t; repeat reduce || simpl_lia.
+  all: try solve [
+      repeat destruct_match; 
+      repeat cps_rec_nf_correct_ind IHn || simpl_lia || invert_constr;
+      unfold CT.next_free; fold CT.next_free; unfold CT.nf_atom;
+      repeat apply max_le || split; auto with lia].
+Qed.
+
+Lemma cps_rec_nf_correct : forall nf t cnt nf' t', 
+  ST.next_free t <= nf -> cnt < nf -> 
+  cps_rec nf t cnt = (nf', t') -> CT.next_free t' <= nf'.
+Proof.
+  eauto using cps_rec_nf_correct_size.
+Qed.
+
+#[global]
+Hint Resolve cps_rec_nf_correct : cps.
+
+Definition cps nf t := 
+  let c := nf in 
+  let a := nf + 1 in
+  let b := CT.Halt (CT.Var a) in 
+  let cnt := CT.Cnt1 c a b in
+  let (_, t') := cps_rec (nf + 2) t c in 
+  CT.LetC cnt t'.
+
+Fixpoint cpsᵥ (nf : nat) (v : SV.value) {struct v} : nat * CV.value :=
   match v with 
   | SV.Lit l => (nf, CV.Lit l)
   | SV.Tuple v1 v2 => 
-      let (nf1, v1') := cps_rec_v nf v1 in
-      let (nf2, v2') := cps_rec_v nf v2 in
-      (nf2, CV.Tuple v1' v2')
+      let (nf, v1') := cpsᵥ nf v1 in
+      let (nf, v2') := cpsᵥ nf v2 in
+      (nf, CV.Tuple v1' v2')
   | SV.Left v => 
-      let (nf1, v') := cps_rec_v nf v in
-      (nf1, CV.Left v')
+      let (nf, v') := cpsᵥ nf v in
+      (nf, CV.Left v')
   | SV.Right v => 
-      let (nf1, v') := cps_rec_v nf v in
-      (nf1, CV.Right v')
+      let (nf, v') := cpsᵥ nf v in
+      (nf, CV.Right v')
   | SV.Fun (ST.Fnt fname farg fbody) env => 
       let fix cps_rec_v_env nf env := 
         match env with
         | nil => (nf, nil)
         | (n, v) :: env => 
-            let (nf', v') := cps_rec_v nf v in
-            let (nf'', env') := cps_rec_v_env nf' env in
-            (nf'', (n, v') :: env')
+            let (nf, v') := cpsᵥ nf v in
+            let (nf, env) := cps_rec_v_env nf env in
+            (nf, (n, v') :: env)
         end in
-      let (nf', env') := cps_rec_v_env nf env in
-      let retC := nf' in
-      let (nf'', fbody') := cps_rec (nf' + 1) fbody (fun r =>
-        let (nf0, res) := r in
-        (nf0, CPS.Tree.AppC1 retC res)
-      ) in
-      (nf'', CV.Fun (CPS.Tree.Fnt fname retC farg fbody') env')
+      let (nf, env) := cps_rec_v_env nf env in
+      let c := nf in
+      let (nf, fbody) := cps_rec (nf + 1) fbody c in
+      (nf, CV.Fun (CT.Fnt fname c farg fbody) env)
   end.
+
+Definition equivᵥ nf v1 v2 := exists e, (e = { } \/ nf <= min e) /\ v1 = renameᵥ e v2.
+
+Lemma cps_v_equiv : forall v nf1 nf2,
+  let (_, v1) := cpsᵥ nf1 v in 
+  let (_, v2) := cpsᵥ nf2 v in 
+    equivᵥ nf1 v1 v2.
+Proof.
+  induction v; repeat reduce || destruct_match.
+  - eexists; reduce.
+  - pose proof (IHv1 nf1 nf2).
+    pose proof (IHv2 n2 n1).
+    repeat reduce || destruct_match.
+    unfold equivᵥ in H, H0.
+    repeat destruct_exist_H || destruct_and_H.
+    repeat destruct_or_H; subst.
+    * exists { }.
+      repeat rewrite rename_v_empty in *.
+      reduce.
+    *  
+
+    
+    
+
+Lemma cps_v_equiv : forall v nf1 nf2,
+  let (_, v1) := cpsᵥ nf1 v in 
+  let (_, v2) := cpsᵥ nf2 v in 
+    v1 ≡ᵥ v2.
+Proof with eauto with equiv_cps.
+  induction v; repeat reduce || destruct_match...
+  - (* Tuple *)
+    specialize (IHv1 nf1 nf2).
+    specialize (IHv2 nf1 nf2).
+    repeat destruct_match || destruct_exist_H || reduce.
+
+Fixpoint cps_envᵥ (nf : nat) (env : env SV.value) := 
+  match env with 
+  | nil => (nf, nil) 
+  | (n, v)::env => 
+      let (nf', v') := cpsᵥ nf v in 
+      let (nf'', env') := cps_envᵥ nf' env in 
+      (nf'', (n, v')::env')
+  end.
+
+Lemma cps_env_keep_elem : forall env nf1 nf2 n v,
+  env ? n = Some v -> 
+  let (_, env') := cps_envᵥ nf1 env in 
+  let (_, v2) := cpsᵥ nf2 v in 
+    exists v1 k, 
+      env' ? n = Some v1 /\ v1 ≡ᵥ v2 @ k.
+Proof. 
+  induction env.
+  - (* nil *) 
+    repeat reduce.
+  - destruct a; repeat reduce || destruct_match.
+    + exists v.
+
+
+Theorem cps_rec_correct : forall f t v io env io',
+    evalₛ f env t io = (Rval v, io') -> forall nf c a b cenvV cenvC, 
+    ST.next_free_env env <= nf -> ST.next_free t <= nf ->
+    c < nf -> a < nf ->  CT.next_free b <= nf -> 
+    CV.next_free_envV cenvV <= nf -> CV.next_free_envC cenvC <= nf -> 
+      let cnt := Cnt (Cnt1 c a b) cenvV cenvC in
+      let (nf', t') := cps_rec nf t c in 
+      let (nf'', v') := cpsᵥ nf' v in 
+      let (_, envV) := cps_envᵥ nf'' env in
+      forall f1 envC,
+        let (r1, io1) := evalₜ f1 envV (envC + (c, cnt)) t' io in 
+        exists f2 k,
+          let (r2, io2) := evalₜ f2 (envV + (a, v')) (envC + (c, cnt)) b io in 
+            io1 = io2 /\ r1 ≡ᵣ r2 @ k.
+Proof. 
+  induction f, t; inversion 1; repeat reduce || destruct_match.
+  - (* Var n *) 
+    destruct f1 eqn:F; repeat reduce.
+    + exists 0, 0; repeat reduce; auto with equiv_cps.
+    + enough (c =? c = true).
+      rewrite H in *.
+      autorewrite*.
+      
+(* 
+Theorem cps_rec_correct_timeout : forall f t io env io', 0 < f -> 
+  evalₛ f env t io = (SV.Rtimeout, io') -> forall nf cnt ca cb envV envC, 
+    ST.next_free t <= nf -> next_free_env env <= nf -> cnt < nf ->
+    let (nf', env') := cps_envᵥ nf env in 
+    let (_, t') := cps_rec nf' t cnt in 
+    exists f', 0 < f' -> 
+      evalₜ f' env' (empty + (cnt, Cnt (Cnt1 cnt ca cb) envV envC)) t' io = (Rtimeout, io').
+Proof.
+  induction f, t; try lia.
+  all: repeat reduce || destruct_match || simpl_lia.
+  - 
+  all: eexists.
+
+
+Theorem cps_correct_ind : forall t v io env f io',
+  evalₛ f env t io = (Rval v, io') -> 
+  ST.next_free t <= nf -> cnt < nf ->
+
+Theorem cps_correct : forall t v io env f io',
+  let nf := max (next_free t) (max (next_free_env env) (next_freeᵥ v)) in
+  { io | env } t ~>(f) { Rval v, io' } ->
+  exists v' f', snd (cpsᵥ nf v) ≡ᵥ v' /\
+    { io | (snd (cps_envᵥ nf env), empty) } snd (cps nf t) ~>(f') { Rhalt v', io' }.
+Proof.
+  intros.
+  induction H; simpl. *)
