src/CPS/Equi.v
@@ -1,8 +1,693 @@
 From Utils Require Import Tactics Env.
 From CPS Require Import Tree Fun_sem.
 
+(* (* Section Term_rel.
+  Variable val_rel : nat -> value -> value -> Prop.
+
+  Definition res_rel' (k : nat) (r1 r2 : result): Prop := 
+    match r1, r2 with 
+    | Rtimeout, Rtimeout => True
+    | Rerr, Rerr => True
+    | Reoi, Reoi => True
+    | Rhalt v1, Rhalt v2 => val_rel k v1 v2 
+    | _, _ => False
+    end.
+
+  Definition term_rel' (k : nat) (e1 e2 : env value * env cntV * term): Prop :=
+    let '(Γ1, Γc1, t1) := e1 in 
+    let '(Γ2, Γc2, t2) := e2 in 
+      forall k' io io1 io2 r1 r2, k' < k -> 
+        evalₜ k' Γ1 Γc1 t1 io = (r1, io1) -> 
+        evalₜ k' Γ2 Γc2 t2 io = (r2, io2) ->
+          res_rel' (k - k') r1 r2 /\ io1 = io2.
+End Term_rel.
+
+Section Cnt_rel.
+  Variable val_rel : nat -> value -> value -> Prop.
+
+  Definition cnt_rel' (k : nat) (cnt1 cnt2 : cntV) : Prop :=
+    match cnt1, cnt2 with
+    | Cnt (Cnt0 n1 b1) Γ1 Γc1, Cnt (Cnt0 n2 b2) Γ2 Γc2 => 
+        let Γc1' := Γc1 + (n1, cnt1) in 
+        let Γc2' := Γc2 + (n2, cnt2) in 
+        term_rel' val_rel k (Γ1, Γc1', b1) (Γ2, Γc2', b2)
+    | Cnt (Cnt1 n1 a1 b1) Γ1 Γc1, Cnt (Cnt1 n2 a2 b2) Γ2 Γc2 => 
+        forall v1 v2, val_rel k v1 v2 -> 
+          let Γ1' := Γ1 + (a1, v1) in 
+          let Γc1' := Γc1 + (n1, cnt1) in 
+          let Γ2' := Γ2 + (a2, v2) in 
+          let Γc2' := Γc2 + (n2, cnt2) in 
+          term_rel' val_rel k (Γ1', Γc1', b1) (Γ2', Γc2', b2)
+    | _ , _ => False
+    end.
+End Cnt_rel.
+
+Fixpoint val_rel (k : nat) (v1 v2 : value) {struct k}: Prop :=
+  let fix val_rel_aux (v1 v2 : value) {struct v1}: Prop :=
+    match v1, v2 with
+    | Lit l1, Lit l2 => l1 = l2
+    | Tuple v1_1 v1_2, Tuple v2_1 v2_2 =>
+        val_rel_aux v1_1 v2_1 /\ val_rel_aux v1_2 v2_2
+    | Left v1, Left v2 =>
+        val_rel_aux v1 v2
+    | Right v1, Right v2 =>
+        val_rel_aux v1 v2
+    | Fun (Fnt n1 c1 a1 b1) Γ1, Fun (Fnt n2 c2 a2 b2) Γ2 =>
+        match k with
+        | 0 => True 
+        | S k' => 
+            forall v1' v2' ac1 bc1 Γc1 Γcnt1 ac2 bc2 Γc2 Γcnt2,
+              let cnt1 := Cnt (Cnt1 c1 ac1 bc1) Γc1 Γcnt1 in
+              let cnt2 := Cnt (Cnt1 c2 ac2 bc2) Γc2 Γcnt2 in
+              let Γ1' := Γ1 + (n1, v1) + (a1, v1') in
+              let Γ2' := Γ2 + (n2, v2) + (a2, v2') in
+              let Γc1' := empty + (c1, cnt1) in
+              let Γc2' := empty + (c2, cnt2) in
+              val_rel k' v1' v2' ->
+              cnt_rel' val_rel k' cnt1 cnt2 -> 
+                term_rel' val_rel k' (Γ1', Γc1', b1) (Γ2', Γc2', b2)
+        end
+    | _, _ => False
+    end
+  in val_rel_aux v1 v2.
+
+Notation res_rel := (res_rel' val_rel).
+
+Notation term_rel := (term_rel' val_rel).
+
+Notation cnt_rel := (cnt_rel' val_rel).
+
+Opaque val_rel.
+
+Lemma res_rel_montone : 
+  (forall k v1 v2, val_rel k v1 v2 -> val_rel (S k) v1 v2) -> 
+    (forall k r1 r2, res_rel k r1 r2 -> res_rel (S k) r1 r2).
+Proof.
+  induction k, r1, r2; simpl; auto.
+Qed.
+
+Lemma eval_0_timeout : forall Γ Γc t io, 
+  evalₜ 0 Γ Γc t io = (Rtimeout, io).
+Proof.
+  auto.
+Qed.
+
+Ltac apply_eval_0_timeout := 
+  match goal with
+  | H : evalₜ 0 _ _ _ _ = (_, _) |- _ =>
+      rewrite eval_0_timeout in H; invert_constr
+  end.
+
+Opaque evalₜ.
+
+Lemma term_rel_monotone : 
+  (forall k v1 v2, val_rel k v1 v2 -> val_rel (S k) v1 v2) -> 
+    (forall k e1 e2, term_rel k e1 e2 -> term_rel (S k) e1 e2).
+Proof.
+  induction k; destruct e1 as [[? ?] ?], e2 as [[? ?] ?]; destruct t, t0.
+  all: simpl in *; intros.
+  all: destruct k'; repeat apply_eval_0_timeout; try lia.
+  all: repeat reduce; simpl_lia.
+  all: pose proof (H0 A)
+  eapply H0 in A.
+  - unfold evalₜ in *. 
+
+Lemma res_rel_refl_aux : 
+  (forall k v, val_rel k v v) -> (forall k r, res_rel k r r).
+Proof.
+  intros; induction r; simpl; auto.
+Qed.
+
+Lemma term_rel_refl_aux : 
+  (forall k v, val_rel k v v) -> (forall k e, term_rel k e e).
+Proof.
+  intros; induction k; destruct e as [[Γ Γc] t]; simpl; auto with lia.
+  intros. exists k', r1; intuition auto.
+  fold res_rel. auto using res_rel_refl_aux.
+Qed.
+
+Lemma eval_env_rel : 
+
+
+Lemma cnt_rel_refl_aux : 
+  (forall k v, val_rel k v v) -> (forall k cnt, cnt_rel k cnt cnt).
+Proof.
+  intros; destruct cnt; destruct cnt; repeat reduce.
+  - (* Cnt0 *)
+    exists k', r1; fold res_rel. intuition auto using res_rel_refl_aux.
+  - exists k', r1; fold res_rel. intuition auto using res_rel_refl_aux.
+  
+
+
+Section value_rel.
+  Variable term_rel : nat -> env value * env cntV * term -> env value * env cntV * term -> Prop.
+  Variable cps_rel : nat -> cntV -> cntV -> Prop.
+  
+  Notation "e1 '≡ₜ' e2 '@' k" := (term_rel k e1 e2) (at level 70, no associativity).
+  Notation "cnt1 '≡ᵧ' cnt2 '@' k" := (cps_rel k cnt1 cnt2) (at level 70, no associativity).
+
+  Definition val_sub (v1 v2 : value) : Prop :=
+    match v2 with
+    | Tuple v2_1 v2_2 => v1 = v2_1 \/ v1 = v2_2
+    | Left v2 => v1 = v2 
+    | Right v2 => v1 = v2 
+    | _ => False
+    end.
+
+  Definition arg_lt (a1 a2 : nat * value) := 
+    match a1, a2 with
+    | (k1, v1), (k2, v2) => k1 < k2 \/ val_sub v1 v2
+    end.
+
+  Require Import Program Program.Wf.
+
+  Program Fixpoint val_rel' (a : nat * value) (v2 : value) { wf arg_lt a } : Prop := 
+    let (k, v1) := a in 
+    match v1, v2 with
+    | Lit l1, Lit l2 => l1 = l2 
+    | Tuple v1_1 v1_2, Tuple v2_1 v2_2 =>
+        val_rel' (k, v1_1) v2_1 /\ val_rel' (k, v1_2) v2_2
+    | Left v1, Left v2 =>
+        val_rel' (k, v1) v2 
+    | Right v1, Right v2 =>
+        val_rel' (k, v1) v2
+    | Fun (Fnt n1 c1 a1 b1) Γ1, Fun (Fnt n2 c2 a2 b2) Γ2 => 
+        forall v1' v2' ac1 bc1 Γc1 Γcnt1 ac2 bc2 Γc2 Γcnt2, 
+          let Γ1' := Γ1 + (n1, v1) + (a1, v1') in 
+          let cnt1 := Cnt (Cnt1 c1 ac1 bc1) Γc1 Γcnt1 in
+          let Γc1' := empty + (c1, cnt1) in 
+          let Γ2' := Γ2 + (n2, v2) + (a2, v2') in 
+          let cnt2 := Cnt (Cnt1 c2 ac2 bc2) Γc2 Γcnt2 in
+          let Γc2' := empty + (c2, cnt2) in 
+          val_rel' (k, v1') v2' ->
+          cnt1 ≡ᵧ cnt2 @ k -> 
+            (Γ1', Γc1', b1) ≡ₜ (Γ2', Γc2', b2) @ k
+    | _, _ => False
+    end.
+  Obligation 1.
+    
+  Defined.
+    
+    Print val_rel'.
+
+  Definition val_rel (k : nat) (v1 v2 : value) : Prop :=
+    val_rel' (k, v1) v2.
+  
+
+  Function val_rel (k : nat) (v1 v2 : value) {struct k} : Prop := 
+    match v1, v2 with 
+    | Lit l1, Lit l2 => l1 = l2 
+    | Tuple v1_1 v1_2, Tuple v2_1 v2_2 => 
+        (* v1_1 ≡ᵥ v2_1 @ k /\ v1_2 ≡ᵥ v2_2 @ k *)
+        val_rel k v1_1 v2_1 /\ val_rel k v1_2 v2_2
+    | Left v1, Left v2 => 
+        (* v1 ≡ᵥ v2 @ k *)
+        val_rel k v1 v2
+    | Right v1, Right v2 => 
+        (* v1 ≡ᵥ v2 @ k *)
+        val_rel k v1 v2
+    | Fun (Fnt n1 c1 a1 b1) Γ1, Fun (Fnt n2 c2 a2 b2) Γ2 => 
+        let f1 := Fnt n1 c1 a1 b1 in 
+        let f2 := Fnt n2 c2 a2 b2 in
+        forall v1' v2' ac1 bc1 Γc1 Γcnt1 ac2 bc2 Γc2 Γcnt2, 
+          (* v1' ≡ᵥ v2' @ k ->  *)
+          val_rel k v1' v2' ->
+          let Γ1' := Γ1 + (n1, v1) + (a1, v1') in 
+          let cnt1 := Cnt1 c1 ac1 bc1 in
+          let Γc1 := empty + (c1, Cnt cnt1 Γc1 Γcnt1) in 
+          let Γ2' := Γ2 + (n2, v2) + (a2, v2') in 
+          let cnt2 := Cnt1 c2 ac2 bc2 in
+          let Γc2 := empty + (c2, Cnt cnt2 Γc2 Γcnt2) in 
+            (Γ1', Γc1, b1) ≡ₜ (Γ2', Γc2, b2) @ k
+    | _, _ => False
+    end.
+  "v1 ≡ᵥ v2 @ k" := (val_rel k v1 v2). *)
+
+  Inductive equiv_v : nat -> value -> value -> Prop := 
+    | lit_rel : forall k l, Lit l ≡ᵥ Lit l @ k
+    | equiv_tuple : forall k v1 v1' v2 v2', 
+        v1 ≡ᵥ v2 @ k -> v1' ≡ᵥ v2' @ k -> Tuple v1 v1' ≡ᵥ Tuple v2 v2' @ k
+    | equiv_left : forall k v1 v2, 
+        v1 ≡ᵥ v2 @ k -> Left v1 ≡ᵥ Left v2 @ k
+    | equiv_right : forall k v1 v2, 
+        v1 ≡ᵥ v2 @ k -> Right v1 ≡ᵥ Right v2 @ k
+    | equiv_fun : forall k n1 c1 a1 b1 Γ1 n2 c2 a2 b2 Γ2 ac bc Γc Γcnt,
+        let f1 := Fnt n1 c1 a1 b1 in 
+        let cnt1 := Cnt1 c1 ac bc in
+        let Γ1' := Γ1 + (n1, Fun f1 Γ1) in 
+        let Γc1 := empty + (c1, Cnt cnt1 Γc Γcnt) in 
+        let f2 := Fnt n2 c2 a2 b2 in 
+        let cnt2 := Cnt1 c2 ac bc in
+        let Γ2' := Γ2 + (n2, Fun f2 Γ2) in 
+        let Γc2 := empty + (c2, Cnt cnt2 Γc Γcnt) in 
+        (forall v1 v2, v1 ≡ᵥ v2 @ k ->
+        (* (forall k' v, k' < k -> )*)
+          (Γ1' + (a1, v1), Γc1, b1) ≡ₜ (Γ2' + (a2, v2), Γc2, b2) @ k) ->
+            Fun f1 Γ1 ≡ᵥ Fun f2 Γ2 @ S k
+  where "v1 '≡ᵥ' v2 '@' k" := (equiv_v k v1 v2). *)
+
+Section Equiv_env.
+  Variable equiv_v : nat -> value -> value -> Prop.
+
+  Definition equiv_env' (k m : nat) (e1 e2 : env value) : Prop :=
+    forall k, m <= k -> forall v1, 
+      e1 ? k = Some v1 -> exists v2, e2 ? k = Some v2 /\ equiv_v k v1 v2.
+End Equiv_env.
+
+Section Equiv_t.
+  Variable equiv_v : nat -> value -> value -> Prop.
+
+  Definition equiv_r' (k : nat) (r1 r2 : result) : Prop := 
+    match r1, r2 with
+    | Rtimeout, Rtimeout => True
+    | Rerr, Rerr => True
+    | Reoi, Reoi => True
+    | Rhalt v1, Rhalt v2 => equiv_v k v1 v2
+    | _, _ => False
+    end.
+  
+  Definition equiv_t' (k : nat) (e1 e2 : env value * env cntV * term): Prop :=
+    let '(Γ1, Γc1, t1) := e1 in 
+    let '(Γ2, Γc2, t2) := e2 in 
+      forall io r1 r2 io1 io2 f1 f2,  
+        evalₜ k Γ1 Γc1 t1 io = (r1, io1, f1) -> 
+        evalₜ k Γ2 Γc2 t2 io = (r2, io2, f2) ->
+          f1 = f2 /\ equiv_r' f1 r1 r2 /\ io1 = io2.
+End Equiv_t.
+
+Section Equiv_c.
+  Variable equiv_v : nat -> value -> value -> Prop.
+
+  Definition equiv_c' (k : nat) (cnt1 cnt2 : cntV) : Prop :=
+    match cnt1, cnt2 with
+    | Cnt (Cnt0 n1 b1) Γ1 Γc1, Cnt (Cnt0 n2 b2) Γ2 Γc2 => 
+        let Γc1' := Γc1 + (n1, cnt1) in 
+        let Γc2' := Γc2 + (n2, cnt2) in 
+        equiv_t' equiv_v k (Γ1, Γc1', b1) (Γ2, Γc2', b2)
+    | Cnt (Cnt1 n1 a1 b1) Γ1 Γc1, Cnt (Cnt1 n2 a2 b2) Γ2 Γc2 => 
+        forall v1 v2, equiv_v k v1 v2 -> 
+          let Γ1' := Γ1 + (a1, v1) in 
+          let Γc1' := Γc1 + (n1, cnt1) in 
+          let Γ2' := Γ2 + (a2, v2) in 
+          let Γc2' := Γc2 + (n2, cnt2) in 
+            equiv_t' equiv_v k (Γ1', Γc1', b1) (Γ2', Γc2', b2)
+    | _ , _ => False
+    end.
+End Equiv_c.
+
+Require Import Program.Wf.
+
+Program Fixpoint equiv_v (k : nat) (v1 v2 : value) {struct k}: Prop :=
+  let fix equiv_v_aux (v1 v2 : value) {struct v1}: Prop :=
+    match v1, v2 with
+    | Lit l1, Lit l2 => l1 = l2
+    | Tuple v1_1 v1_2, Tuple v2_1 v2_2 =>
+        equiv_v_aux v1_1 v2_1 /\ equiv_v_aux v1_2 v2_2
+    | Left v1, Left v2 =>
+        equiv_v_aux v1 v2
+    | Right v1, Right v2 =>
+        equiv_v_aux v1 v2
+    | Fun (Fnt n1 c1 a1 b1) Γ1, Fun (Fnt n2 c2 a2 b2) Γ2 =>
+        match k with
+        | 0 => True 
+        | S k' => 
+            forall v1' v2' ac1 bc1 Γc1 Γcnt1 ac2 bc2 Γc2 Γcnt2,
+              let cnt1 := Cnt (Cnt1 c1 ac1 bc1) Γc1 Γcnt1 in
+              let cnt2 := Cnt (Cnt1 c2 ac2 bc2) Γc2 Γcnt2 in
+              let Γ1' := Γ1 + (n1, v1) + (a1, v1') in
+              let Γ2' := Γ2 + (n2, v2) + (a2, v2') in
+              let Γc1' := empty + (c1, cnt1) in
+              let Γc2' := empty + (c2, cnt2) in
+              equiv_v k' v1' v2' ->
+              equiv_c' equiv_v k' cnt1 cnt2 -> 
+                equiv_t' equiv_v k' (Γ1', Γc1', b1) (Γ2', Γc2', b2)
+        end
+    | _, _ => False
+    end
+  in equiv_v_aux v1 v2.
+
+Notation equiv_r := (equiv_r' equiv_v).
+Notation equiv_t := (equiv_t' equiv_v).
+Notation equiv_c := (equiv_c' equiv_v).
+
+Notation "r1 '≡ᵣ' r2" := (forall k, equiv_r k r1 r2) (at level 70, no associativity).
+Notation "e1 '≡ₜ' e2" := (forall k, equiv_t k e1 e2) (at level 70, no associativity).
+Notation "c1 '≡ᵧ' c2" := (forall k, equiv_c k c1 c2) (at level 70, no associativity).
+Notation "v1 '≡ᵥ' v2" := (forall k, equiv_v k v1 v2) (at level 70, no associativity).
+
+(* Lemma equiv_v_refl_0 : forall v, 
+  equiv_v 0 v v.
+Proof.
+  induction v; reduce.
+  destruct_match; reduce.
+Qed.
+
+Lemma equiv_r_refl_0 : forall r, 
+  equiv_r 0 r r.
+Proof.
+  induction r; reduce.
+  induction v; reduce.
+  destruct_match; reduce.
+Qed.
+
+Lemma equiv_t_relf_0 : forall t Γ Γc,
+  equiv_t 0 (Γ, Γc, t) (Γ, Γc, t).
+Proof.
+  induction t; reduce.
+Qed.
+
+Lemma equiv_c_refl_0 : forall c, 
+  equiv_c 0 c c.
+Proof.
+  induction c; reduce.
+  destruct_match; reduce.
+Qed.
+
+Lemma equiv_v_refl_1 : forall v, 
+  equiv_v 1 v v.
+Proof.
+  induction v; reduce.
+  destruct_match; reduce.
+Qed.
+
+Lemma equiv_r_refl_1 : forall r, 
+  equiv_r 1 r r.
+Proof.
+  induction r; reduce.
+  apply equiv_v_refl_1.
+Qed.
+
+Lemma equiv_t_relf_1 : forall t Γ Γc,
+  equiv_t 1 (Γ, Γc, t) (Γ, Γc, t).
+Proof.
+  induction t; reduce.
+  all: repeat destruct_match; reduce.
+  apply equiv_v_refl_1.
+Qed.
+
+Lemma bin_op_equiv_v : forall op k v1 v2 e a1 a2 n v1',
+  equiv_v k v1 v2 -> 
+  binary_op_atom (e + (n, v1)) op a1 a2 = Some v1' -> 
+    exists v2', binary_op_atom (e + (n, v2)) op a1 a2 = Some v2'.
+Proof.
+  destruct op, k, a1, a2; reduce; 
+  unfold binary_op_atom, get_value_atom in *.
+  all: repeat reduce || env || destruct_match; eauto.
+Qed.
+
+Lemma bin_op_equiv_v_err : forall op k v1 v2 e a1 a2 n, 
+  equiv_v k v1 v2 -> 
+  binary_op_atom (e + (n, v1)) op a1 a2 = None -> 
+    binary_op_atom (e + (n, v2)) op a1 a2 = None.
+Proof.
+  destruct op, k, a1, a2; reduce;
+  unfold binary_op_atom, get_value_atom in *.
+  all: repeat reduce || env || destruct_match; eauto.
+Qed.
+
+Lemma un_op_equiv_v : forall op k v1 v2 e a n v1', 
+  equiv_v k v1 v2 ->
+  unary_op_atom (e + (n, v1)) op a = Some v1' -> 
+    exists v2', unary_op_atom (e + (n, v2)) op a = Some v2'.
+Proof.
+  destruct op, k, a; reduce;
+  unfold unary_op_atom, get_value_atom in *.
+  all: repeat reduce || env || destruct_match; eauto.
+Qed.
+
+Lemma un_op_equiv_v_err : forall op k v1 v2 e a n,
+  equiv_v k v1 v2 ->
+  unary_op_atom (e + (n, v1)) op a = None -> 
+    unary_op_atom (e + (n, v2)) op a = None.
+Proof.
+  destruct op, k, a; reduce;
+  unfold unary_op_atom, get_value_atom in *.
+  all: repeat reduce || env || destruct_match; eauto.
+Qed.
+
+Lemma equiv_c_refl_1 : forall c, 
+  equiv_c 1 c c.
+Proof.
+  destruct c; reduce.
+  repeat destruct_match; reduce; 
+  try solve [
+    unfold get_value_atom in *;
+    repeat reduce || env || destruct_match
+  ].
+  - apply equiv_v_refl_1.
+  - destruct (binary_op_atom (envV + (arg, v1)) op a1 a2) eqn:E.
+    * pose proof (bin_op_equiv_v op 1 v1 v2 envV a1 a2 arg).
+      apply (H2 v) in H as [v2' ?]; auto.
+      rewrite H in *; reduce.
+    * pose proof (bin_op_equiv_v_err op 1 v1 v2 envV a1 a2 arg).
+      apply H2 in H; auto.
+      rewrite H in *; reduce.
+  - destruct (unary_op_atom (envV + (arg, v1)) op a) eqn:E.
+    * pose proof (un_op_equiv_v op 1 v1 v2 envV a arg).
+      apply (H2 v) in H as [v2' ?]; auto.
+      rewrite H in *; reduce.
+    * pose proof (un_op_equiv_v_err op 1 v1 v2 envV a arg).
+      apply H2 in H; auto.
+      rewrite H in *; reduce.
+  - unfold get_value_atom in *;
+    repeat reduce || env || destruct_match.
+    apply equiv_v_refl_1.
+Qed.
+
+Lemma equiv_v_refl_2 : forall v, 
+  equiv_v 2 v v.
+Proof.
+  induction v; reduce.
+  destruct f; intros.
+  destruct body.
+  - destruct (binary_op_atom (e + (name, Fun (Fnt name retC arg (LetB name0 op a1 a2 body)) e) + (arg, v1')) op a1 a2) eqn:E.
+    * pose proof (bin_op_equiv_v op 1 v1' v2' (e + (name, Fun (Fnt name retC arg (LetB name0 op a1 a2 body)) e)) a1 a2 arg).
+      apply (H3 v) in H as [v' ?]; auto.
+      rewrite H in *; reduce.
+    * pose proof (bin_op_equiv_v_err op 1 v1' v2' (e + (name, Fun (Fnt name retC arg (LetB name0 op a1 a2 body)) e)) a1 a2 arg).
+      apply H3 in H; auto.
+      rewrite H in *; reduce.
+  - destruct (unary_op_atom (e + (name, Fun (Fnt name retC arg (LetU name0 op a body)) e) + (arg, v1')) op a) eqn:E.
+    * pose proof (un_op_equiv_v op 1 v1' v2' (e + (name, Fun (Fnt name retC arg (LetU name0 op a body)) e)) a arg).
+      apply (H3 v) in H as [v' ?]; auto.
+      rewrite H in *; reduce.
+    * pose proof (un_op_equiv_v_err op 1 v1' v2' (e + (name, Fun (Fnt name retC arg (LetU name0 op a body)) e)) a arg).
+      apply H3 in H; auto.
+      rewrite H in *; reduce.
+  - destruct cont; reduce.
+  - destruct f; reduce.
+  - destruct (IO.get_input io); reduce. 
+    destruct p; reduce.
+  - unfold get_value_atom in *.
+    destruct a.
+    * destruct (Nat.eq_dec n0 arg); subst.
+      + rewrite lookup_add_eq in *.
+        destruct v1', v2'; reduce.
+        destruct l0; reduce.
+        destruct f; reduce.
+        destruct f; reduce.
+      + rewrite lookup_add_ne in *; try lia.
+        rewrite H1 in H2; reduce.
+        apply equiv_r_refl_1.
+    * rewrite H1 in H2; reduce.
+      apply equiv_r_refl_1.
+  - destruct (Nat.eq_dec retC name0); subst.
+    * rewrite lookup_add_eq in *; reduce.
+    * rewrite lookup_add_ne in *; try lia.
+      rewrite lookup_empty in *; reduce.
+  - destruct (Nat.eq_dec retC name0); subst.
+    * rewrite lookup_add_eq in *.
+      unfold get_value_atom in *.
+      destruct a.
+
+
+
+    * rewrite lookup_add_ne in *; try lia.
+      rewrite lookup_empty in *; reduce.
+
+    
+    
+    
+    destruct_match; reduce.
+  - unfold get_value_atom in *.
+    destruct a.
+    * destruct (Nat.eq_dec n0 arg); reduce.
+      + rewrite lookup_add_eq in *.
+        destruct v1', v2'; reduce.
+        destruct l0; reduce.
+        destruct f; reduce.
+      + rewrite lookup_add_ne in *; try lia.
+        destruct (Nat.eq_dec n0 name); reduce. {
+          rewrite lookup_add_eq in *; reduce.
+        } {
+          rewrite lookup_add_ne in *; try lia.
+          repeat reduce || destruct_match.
+        }
+    * destruct lit; reduce.
+  - unfold get_value_atom in *.
+    destruct a.
+    * destruct (Nat.eq_dec n0 arg); reduce.
+      + rewrite lookup_add_eq in *.
+        destruct v1', v2'; reduce.
+        destruct f; reduce.
+      + rewrite lookup_add_ne in *; try lia.
+        destruct (Nat.eq_dec n0 name); reduce.
+    * destruct lit; reduce.
+  - repeat reduce || env. 
+  - repeat reduce || env. 
+  - destruct (Nat.eq_dec retC name0); reduce.
+    * rewrite lookup_add_eq in *.
+      unfold get_value_atom in *.
+      destruct a; reduce.
+
+      env.
+    
+    repeat reduce || env. 
+
+
+Lemma eval_equiv_env : forall k 
+
+Lemma eval_equiv_v : forall k t Γ Γc io n v1 v2 r1 r2 io1 io2, equiv_v k v1 v2 ->
+  evalₜ k (Γ + (n, v1)) Γc t io = (r1, io1) ->
+  evalₜ k (Γ + (n, v2)) Γc t io = (r2, io2) ->
+    equiv_r k r1 r2 /\ io1 = io2.
+Proof.
+  induction k, t; inversion 2; inversion 1; try solve [reduce].
+  - destruct (Nat.eq_dec n name).
+    * reduce.
+      rewrite add_dup in H4.
+    env.
+  - reduce.  
+
+Lemma equiv_v_refl_0 : forall v, equiv_v 0 v v.
+Proof.
+  induction v; repeat reduce || destruct_match.
+Qed.
+
+Lemma equiv_v_refl : forall k v, equiv_v k v v.
+Proof. 
+  induction v, k; auto using equiv_v_refl_0; reduce.
+  destruct_match; reduce.
+  - reduce.
+  - reduce.
+  - simpl. 
+    apply (IHk v1).
+    unfold equiv_v.
+    repeat reduce || destruct_match.
+  all: reduce. 
+  - apply (IHv1 0).
+  - apply (IHv2 0).
+  - apply (IHv1 (S k)).
+  - apply (IHv2 (S k)).
+  - apply (IHv 0).
+  - apply (IHv (S k)).
+  - apply (IHv 0).
+  - apply (IHv (S k)).
+  - repeat reduce || destruct_match.
+  - repeat reduce || destruct_match.
+
+    admit.
+Admitted.
+
+Lemma value_eqb_equiv_v : forall v1 v2, value_eqb v1 v2 = true -> v1 ≡ᵥ v2.
+Proof.
+  induction v1; destruct v2; reduce.
+  - destruct l, l0, k; reduce; f_equal.
+    1, 2: apply BinInt.Z.eqb_eq in H; auto.
+    all: apply Bool.eqb_prop in H; auto.
+  - apply andb_prop in H. 
+    destruct_and_H.
+    pose proof (IHv1_1 _ H k).
+    pose proof (IHv1_2 _ H0 k).
+    destruct k; reduce.
+  - pose proof (IHv1 _ H k).
+    destruct k; reduce.
+  - pose proof (IHv1 _ H k).
+    destruct k; reduce.
+Qed.
+
+Lemma equiv_v_binary : forall k n v1 v2 env op a1 a2, equiv_v k v1 v2 -> 
+  forall v1', binary_op_atom (env + (n, v1)) op a1 a2 = Some v1' ->
+    exists v2', binary_op_atom (env + (n, v2)) op a1 a2 = Some v2' /\ equiv_v k v1' v2'.
+Proof.
+  induction v1, v2, k; reduce.
+  - eexists; reduce; try eassumption. 
+    apply (equiv_v_refl v1' 0).
+  - eexists; reduce; try eassumption. 
+    apply (equiv_v_refl v1' (S k)).
+  - destruct_and_H.
+    eapply IHv1_1 in H. 
+
+  induction k, v1, v2; reduce.
+  - destruct a1, a2; 
+    unfold binary_op_atom, get_value_atom in *;
+    repeat env || reduce || destruct_match || discriminate.
+    all: exists v1'; reduce.
+    all: apply (equiv_v_refl v1' 0).
+  - destruct a1, a2, op; 
+    unfold binary_op_atom, get_value_atom, compute_binary_op in *;
+    repeat env || reduce || destruct_match || discriminate.
+    all: eexists; repeat reduce. 
+    all: try eapply (equiv_v_refl _ 0).
+    all: f_equal.
+    * 
+      destruct v1_1, v1_2, v2_1, v2_2; reduce.
+      all: repeat destruct_and_H || reduce || rewrite lit_eqb_refl.
+    all: intuition eauto.
+    all: exists v1'; reduce.
+
+Lemma equiv_v_binary_err : forall k n v1 v2 env op a1 a2, equiv_v k v1 v2 -> 
+  binary_op_atom (env + (n, v1)) op a1 a2 = None /\ 
+  binary_op_atom (env + (n, v2)) op a1 a2 = None.
+
+
+Lemma equiv_v_t_ind : forall k k' t envV envC n v1 v2 r1 r2 io io', k < k' -> 
+  v1 ≡ᵥ v2 -> 
+  evalₜ k (envV + (n, v1)) envC t io = (r1, io') ->
+  evalₜ k (envV + (n, v2)) envC t io = (r2, io') -> 
+    equiv_r (k - k') r1 r2.
+Proof.
+  induction k; reduce; try lia.
+  destruct k'; simpl_lia.
+  destruct t; reduce.
+  - 
+  
+
+Opaque equiv_v.
+Lemma equiv_r_refl : 
+  (forall k v, equiv_v k v v) -> (forall k r, equiv_r k r r).
+Proof.
+  induction k, r; simpl; auto.
+Qed.
+
+Ltac destruct_eval := 
+  match goal with
+  | H : evalₜ ?f ?Γ ?Γc ?t ?io = (_,  _) |- _ =>
+      let E := fresh "evalₜ" in 
+      destruct (evalₜ f Γ Γc t io) eqn:E
+  end.
+
+Opaque minus.
+
+Lemma equiv_t_relf : 
+  (forall k v, equiv_v k v v) -> (forall k e, equiv_t k e e).
+Proof.
+  induction k, e; destruct p; induction t; simpl in *.
+  all: intros; try lia.
+  all: destruct_eval; repeat invert_constr; intuition auto using equiv_r_refl.
+Qed.
+
+Lemma equiv_c_refl: 
+  (forall k v, equiv_v k v v) -> (forall k c, equiv_c k c c).
+Proof.
+  induction k, c; destruct cnt; simpl in *.
+  all: intros; try lia.
+  all: destruct_eval; repeat invert_constr; intuition auto using equiv_r_refl, equiv_t_relf.
+
+
 Reserved Notation "v1 '≡ᵥ' v2 '@' k" (at level 70, no associativity).
 Reserved Notation "r1 '≡ᵣ' r2 '@' k" (at level 70, no associativity).
+Reserved Notation "e1 '≡ₜ' e2 '@' k" (at level 70, no associativity).  
 
 Inductive equiv_v : nat -> value -> value -> Prop := 
   | equiv_lit : forall k l, Lit l ≡ᵥ Lit l @ k 
@@ -12,27 +697,38 @@ Inductive equiv_v : nat -> value -> value -> Prop :=
       v1 ≡ᵥ v2 @ k -> Left v1 ≡ᵥ Left v2 @ k
   | equiv_right : forall k v1 v2, 
       v1 ≡ᵥ v2 @ k -> Right v1 ≡ᵥ Right v2 @ k
-  | equiv_fun : forall k n1 c1 a1 b1 Γ1 n2 c2 a2 b2 Γ2,
+  | equiv_fun : forall k n1 c1 a1 b1 Γ1 n2 c2 a2 b2 Γ2 ac bc Γc Γcnt,
       let f1 := Fnt n1 c1 a1 b1 in 
+      let cnt1 := Cnt1 c1 ac bc in
+      let Γ1' := Γ1 + (n1, Fun f1 Γ1) in 
+      let Γc1 := empty + (c1, Cnt cnt1 Γc Γcnt) in 
       let f2 := Fnt n2 c2 a2 b2 in 
-      (forall k' io io1 io2 v ac bc Γc Γcnt r1 r2, k' < k -> 
-        let cnt1 := Cnt1 c1 ac bc in
-        let cnt2 := Cnt1 c2 ac bc in
-        evalₜ k' (Γ1 + (n1, Fun f1 Γ1) + (a1, v)) (empty + (c1, Cnt cnt1 Γc Γcnt)) b1 io = (r1, io1) -> 
-        evalₜ k' (Γ2 + (n2, Fun f2 Γ2) + (a2, v)) (empty + (c2, Cnt cnt2 Γc Γcnt)) b2 io = (r2, io2) -> 
-          r1 ≡ᵣ r2 @ k' /\ io1 = io2) -> 
-        Fun f1 Γ1 ≡ᵥ Fun f2 Γ2 @ k
+      let cnt2 := Cnt1 c2 ac bc in
+      let Γ2' := Γ2 + (n2, Fun f2 Γ2) in 
+      let Γc2 := empty + (c2, Cnt cnt2 Γc Γcnt) in 
+      (forall v1 v2, v1 ≡ᵥ v2 @ k ->
+      (* (forall k' v, k' < k -> *)
+        (Γ1' + (a1, v1), Γc1, b1) ≡ₜ (Γ2' + (a2, v2), Γc2, b2) @ k) ->
+          Fun f1 Γ1 ≡ᵥ Fun f2 Γ2 @ S k
 with equiv_r : nat -> result -> result -> Prop :=
   | equiv_halt : forall k v1 v2, 
       v1 ≡ᵥ v2 @ k -> Rhalt v1 ≡ᵣ Rhalt v2 @ k
   | equiv_err : forall k, Rerr ≡ᵣ Rerr @ k
   | equiv_eoi : forall k, Reoi ≡ᵣ Reoi @ k
   | equiv_timeout : forall k, Rtimeout ≡ᵣ Rtimeout @ k
+with equiv_t : nat -> env value * env cntV * term -> env value * env cntV * term -> Prop := 
+  | equiv_eval : forall k Γ1 Γ2 Γc1 Γc2 t1 t2,
+      (forall k1 io io1 r1, k1 < k -> 
+      evalₜ k1 Γ1 Γc1 t1 io = (r1, io1) -> 
+        exists k2 io2 r2, 
+          evalₜ k2 Γ2 Γc2 t2 io = (r2, io2) /\ io1 = io2 /\ r1 ≡ᵣ r2 @ (k1)) ->
+            (Γ1, Γc1, t1) ≡ₜ (Γ2, Γc2, t2) @ k
 where "v1 '≡ᵥ' v2 '@' k" := (equiv_v k v1 v2) and
-      "r1 '≡ᵣ' r2 '@' k" := (equiv_r k r1 r2).
+      "r1 '≡ᵣ' r2 '@' k" := (equiv_r k r1 r2) and 
+      "e1 '≡ₜ' e2 '@' k" := (equiv_t k e1 e2).
 
 #[global]
-Hint Constructors equiv_v equiv_r : equiv_cps.
+Hint Constructors equiv_v equiv_r equiv_t : equiv_cps.
 
 Lemma equiv_fun_0 : forall f1 Γ1 f2 Γ2, 
   Fun f1 Γ1 ≡ᵥ Fun f2 Γ2 @ 0.
@@ -187,4 +883,6 @@ Proof with eauto.
 Qed.
 
 #[global]
-Hint Resolve equiv_v_trans equiv_r_trans : equiv_cps.
+Hint Resolve equiv_v_trans equiv_r_trans : equiv_cps. *)
+
+(* Lemma equiv_monotone : forall k  *)
